Clean up coq structure

doc/coq/Abstract.v
@@ -1,12 +1,12 @@
-Require Export Modular.Syntax.
+From MODULAR Require Export Syntax.
 
-Definition time := nat.
+Definition time := bool.
 
 Definition path := list time.
 
-Definition update_t (t : time) := S t.
+Definition update_t (t : time) := negb t.
 
-Definition eq_t (t1 t2 : time) := t1 =? t2.
+Definition eq_t (t1 t2 : time) := Bool.eqb t1 t2.
 
 Fixpoint eq_p (p1 p2 : path) :=
   match p1, p2 with
@@ -19,6 +19,18 @@ Fixpoint eq_p (p1 p2 : path) :=
   end.
 
 Definition len_p (p : path) := List.length p.
+
+Lemma eq_t_eq :
+  forall t1 t2, eq_t t1 t2 = true <-> t1 = t2.
+Proof.
+  unfold eq_t. apply Bool.eqb_true_iff.
+Qed.
+
+Lemma eq_t_neq :
+  forall t1 t2, eq_t t1 t2 = false <-> t1 <> t2.
+Proof.
+  unfold eq_t. apply Bool.eqb_false_iff.
+Qed.
 
 Inductive dy_ctx :=
   | dy_c_hole
@@ -33,16 +45,6 @@ Fixpoint dy_plugin_c Cout Cin :=
   | dy_c_lam x tx C' => dy_c_lam x tx (dy_plugin_c C' Cin)
   | dy_c_lete x tx C' => dy_c_lete x tx (dy_plugin_c C' Cin)
   | dy_c_letm M CM C' => dy_c_letm M CM (dy_plugin_c C' Cin)
-  end.
-
-Definition eq_eid id1 id2 :=
-  match id1, id2 with
-  | eid x1, eid x2 => x1 =? x2
-  end.
-
-Definition eq_mid id1 id2 :=
-  match id1, id2 with
-  | mid M1, mid M2 => M1 =? M2
   end.
 
 Fixpoint dy_level (C : dy_ctx) : path :=
@@ -98,12 +100,12 @@ Definition update_m {X} mem (p : path) (x : X) :=
 
 Definition empty_mem {X} (p : path) : option X := None.
 
-Notation "p '!->' v ';' mem" := (update_m mem p v)
+Notation "p '!#->' v ';' mem" := (update_m mem p v)
                               (at level 100, v at next level, right associativity).
 
-Notation "Cout '[|' Cin '|]'" := (dy_plugin_c Cout Cin)
+Notation "Cout '[#|' Cin '|#]'" := (dy_plugin_c Cout Cin)
                               (at level 100, Cin at next level, right associativity).
-Notation "'[||]'" := (dy_c_hole) (at level 100).
+Notation "'[#||#]'" := (dy_c_hole) (at level 100).
 
 Inductive EevalR (C : dy_ctx) (st : state)
     : expr_tm -> expr_value -> state -> Prop :=
@@ -124,8 +126,8 @@ Inductive EevalR (C : dy_ctx) (st : state)
                            (Val (e_lam x e) (v_fn x e) C_lam) st_lam)
               (ARG : EevalR C st_lam e2
                             arg (ST mem t))
-              (BODY : EevalR (C_lam [|dy_c_lam x t  ([||])|])
-                             (ST ((dy_level C_lam) ++ [t] !-> arg ; mem) (update_t t))
+              (BODY : EevalR (C_lam [#|dy_c_lam x t ([#||#])|#])
+                             (ST ((dy_level C_lam) ++ [t] !#-> arg ; mem) (update_t t))
                               e v st_v)
     : EevalR C st (e_app e1 e2) v st_v
   | Eeval_link m e C_m st_m v st_v
@@ -142,14 +144,14 @@ with MevalR (C : dy_ctx) (st : state)
   | Meval_lete x e v_e mem t
                m C_m st_m
                (EVALe : EevalR C st e v_e (ST mem t))
-               (EVALm : MevalR (C [|dy_c_lete x t  ([||])|]) 
-                        (ST ((dy_level C ++ [t]) !-> v_e ; mem) (update_t t))
+               (EVALm : MevalR (C [#|dy_c_lete x t ([#||#])|#]) 
+                        (ST ((dy_level C ++ [t]) !#-> v_e ; mem) (update_t t))
                         m C_m st_m)
     : MevalR C st (m_lete x e m) C_m st_m
   | Meval_letm M m1 C_m1 st_m1
                m2 C_m2 st_m2
                (EVALm1 : MevalR C st m1 C_m1 st_m1)
-               (EVALm2 : MevalR (C [|dy_c_letm M C_m1  ([||])|]) st_m1
+               (EVALm2 : MevalR (C [#|dy_c_letm M C_m1 ([#||#])|#]) st_m1
                          m2 C_m2 st_m2)
     : MevalR C st (m_letm M m1 m2) C_m2 st_m2
 .
@@ -190,8 +192,8 @@ Inductive _EreachE (C : dy_ctx) (st : state)
                              (Val (e_lam x e) (v_fn x e) C_lam) st_lam)
                  (ARG : EevalR C st_lam e2
                                arg (ST mem t))
-                 (REACHb : _EreachE (C_lam[|dy_c_lam x t  ([||])|]) 
-                                    (ST ((dy_level C_lam ++ [t]) !-> arg ; mem) (update_t t)) e
+                 (REACHb : _EreachE (C_lam[#|dy_c_lam x t ([#||#])|#]) 
+                                    (ST ((dy_level C_lam ++ [t]) !#-> arg ; mem) (update_t t)) e
                                      C' st' e')
     : _EreachE C st (e_app e1 e2)
                C' st' e'
@@ -217,8 +219,8 @@ with _MreachE (C : dy_ctx) (st : state)
   | _mre_lete_m x e m v mem t
                 C' st' e'
              (EVALx : EevalR C st e v (ST mem t))
-             (REACHm : _MreachE (C[|dy_c_lete x t  ([||])|])
-                                (ST ((dy_level C ++ [t]) !-> v ; mem) (update_t t)) m
+             (REACHm : _MreachE (C[#|dy_c_lete x t ([#||#])|#])
+                                (ST ((dy_level C ++ [t]) !#-> v ; mem) (update_t t)) m
                                  C' st' e')
     : _MreachE C st (m_lete x e m)
                C' st' e'
@@ -230,7 +232,7 @@ with _MreachE (C : dy_ctx) (st : state)
   | _mre_letm_m2 M m1 m2 C_M st_M
                  C' st' e'
              (EVALM : MevalR C st m1 C_M st_M)
-             (REACHm : _MreachE (C[|dy_c_letm M C_M  ([||])|]) st_M m2
+             (REACHm : _MreachE (C[#|dy_c_letm M C_M ([#||#])|#]) st_M m2
                                  C' st' e')
     : _MreachE C st (m_letm M m1 m2)
                C' st' e'.
@@ -254,8 +256,8 @@ Inductive _MreachM (C : dy_ctx) (st : state)
   | _mrm_lete_m x e m v mem t
                 C' st' m'
              (EVALx : EevalR C st e v (ST mem t))
-             (REACHm : _MreachM (C[|dy_c_lete x t  ([||])|]) 
-                                (ST ((dy_level C ++ [t]) !-> v ; mem) (update_t t)) m
+             (REACHm : _MreachM (C[#|dy_c_lete x t ([#||#])|#]) 
+                                (ST ((dy_level C ++ [t]) !#-> v ; mem) (update_t t)) m
                                  C' st' m')
     : _MreachM C st (m_lete x e m)
                C' st' m'
@@ -267,7 +269,7 @@ Inductive _MreachM (C : dy_ctx) (st : state)
   | _mrm_letm_m2 M m1 m2 C_M st_M
                  C' st' m'
              (EVALM : MevalR C st m1 C_M st_M)
-             (REACHm : _MreachM (C[|dy_c_letm M C_M  ([||])|]) st_M m2
+             (REACHm : _MreachM (C[#|dy_c_letm M C_M ([#||#])|#]) st_M m2
                                  C' st' m')
     : _MreachM C st (m_letm M m1 m2)
                C' st' m'
@@ -291,8 +293,8 @@ with _EreachM (C : dy_ctx) (st : state)
                  (FN : EevalR C st e1 
                               (Val (e_lam x e) (v_fn x e) C_lam) st_lam)
                  (ARG : EevalR C st_lam e2 arg (ST mem t))
-                 (REACHb : _EreachM (C_lam[|dy_c_lam x t ([||])|]) 
-                                    (ST ((dy_level C_lam ++ [t]) !-> arg ; mem) (update_t t)) e
+                 (REACHb : _EreachM (C_lam[#|dy_c_lam x t ([#||#])|#]) 
+                                    (ST ((dy_level C_lam ++ [t]) !#-> arg ; mem) (update_t t)) e
                                      C' st' m')
     : _EreachM C st (e_app e1 e2)
                C' st' m'
@@ -346,8 +348,8 @@ Inductive EreachE (C : dy_ctx) (st : state)
                  (ARG : EevalR C st_lam e2
                                (Val arg pf C_arg) (ST mem t))
                  (ARGr : EreachE C st_lam e2 C_arg (ST mem t) arg)
-                 (REACHb : EreachE (C_lam[|dy_c_lam x t ([||])|]) 
-                                    (ST ((dy_level C_lam ++ [t]) !-> (Val arg pf C_arg) ; mem) (update_t t)) e
+                 (REACHb : EreachE (C_lam[#|dy_c_lam x t ([#||#])|#]) 
+                                    (ST ((dy_level C_lam ++ [t]) !#-> (Val arg pf C_arg) ; mem) (update_t t)) e
                                      C' st' e')
     : EreachE C st (e_app e1 e2)
               C' st' e'
@@ -375,8 +377,8 @@ with MreachE (C : dy_ctx) (st : state)
                C' st' e'
              (EVALx : EevalR C st e (Val v pf C_x) (ST mem t))
              (EVALxr : EreachE C st e C_x (ST mem t) v)
-             (REACHm : MreachE (C[|dy_c_lete x t ([||])|])
-                                (ST ((dy_level C ++ [t]) !-> (Val v pf C_x) ; mem) (update_t t)) m
+             (REACHm : MreachE (C[#|dy_c_lete x t ([#||#])|#])
+                                (ST ((dy_level C ++ [t]) !#-> (Val v pf C_x) ; mem) (update_t t)) m
                                  C' st' e')
     : MreachE C st (m_lete x e m)
               C' st' e'
@@ -389,7 +391,7 @@ with MreachE (C : dy_ctx) (st : state)
                 C' st' e'
              (EVALM : MevalR C st m1 C_M st_M)
              (EVALM : MreachM C st m1 C_M st_M m_empty)
-             (REACHm : MreachE (C[|dy_c_letm M C_M ([||])|]) st_M m2
+             (REACHm : MreachE (C[#|dy_c_letm M C_M ([#||#])|#]) st_M m2
                                 C' st' e')
     : MreachE C st (m_letm M m1 m2)
               C' st' e'
@@ -411,8 +413,8 @@ with MreachM (C : dy_ctx) (st : state)
                C' st' m'
              (EVALx : EevalR C st e (Val v pf C_x) (ST mem t))
              (EVALxr : EreachE C st e C_x (ST mem t) v)
-             (REACHm : MreachM (C[|dy_c_lete x t ([||])|]) 
-                               (ST ((dy_level C ++ [t]) !-> (Val v pf C_x) ; mem) (update_t t)) m
+             (REACHm : MreachM (C[#|dy_c_lete x t ([#||#])|#]) 
+                               (ST ((dy_level C ++ [t]) !#-> (Val v pf C_x) ; mem) (update_t t)) m
                                 C' st' m')
     : MreachM C st (m_lete x e m)
               C' st' m'
@@ -425,7 +427,7 @@ with MreachM (C : dy_ctx) (st : state)
                 C' st' m'
              (EVALM : MevalR C st m1 C_M st_M)
              (EVALMr : MreachM C st m1 C_M st_M m_empty)
-             (REACHm : MreachM (C[|dy_c_letm M C_M  ([||])|]) st_M m2
+             (REACHm : MreachM (C[#|dy_c_letm M C_M  ([#||#])|#]) st_M m2
                                 C' st' m')
     : MreachM C st (m_letm M m1 m2)
               C' st' m'
@@ -453,8 +455,8 @@ with EreachM (C : dy_ctx) (st : state)
                                 C_lam st_lam (e_lam x e))
                  (ARG : EevalR C st_lam e2 (Val arg pf C_arg) (ST mem t))
                  (ARGr : EreachE C st_lam e2 C_arg (ST mem t) arg)
-                 (REACHb : EreachM (C_lam[|dy_c_lam x t ([||])|]) 
-                                   (ST ((dy_level C_lam ++ [t]) !-> (Val arg pf C_arg) ; mem) (update_t t)) e
+                 (REACHb : EreachM (C_lam[#|dy_c_lam x t ([#||#])|#]) 
+                                   (ST ((dy_level C_lam ++ [t]) !#-> (Val arg pf C_arg) ; mem) (update_t t)) e
                                     C' st' m')
     : EreachM C st (e_app e1 e2)
               C' st' m'
@@ -477,22 +479,22 @@ with _EreachM_ind_mut := Induction for EreachM Sort Prop
 with _MreachE_ind_mut := Induction for MreachE Sort Prop
 with _MreachM_ind_mut := Induction for MreachM Sort Prop.
 
-Notation "'<e|' C1 st1 tm1 '~>' C2 st2 tm2 '|e>'" := (EreachE C1 st1 tm1 C2 st2 tm2) 
+Notation "'<e|' C1 st1 tm1 '~#>' C2 st2 tm2 '|e>'" := (EreachE C1 st1 tm1 C2 st2 tm2) 
                                                (at level 10, 
                                                 C1 at next level, st1 at next level, tm1 at next level,
                                                 C2 at next level, st2 at next level, tm2 at next level).
 
-Notation "'<m|' C1 st1 tm1 '~>' C2 st2 tm2 '|e>'" := (MreachE C1 st1 tm1 C2 st2 tm2) 
+Notation "'<m|' C1 st1 tm1 '~#>' C2 st2 tm2 '|e>'" := (MreachE C1 st1 tm1 C2 st2 tm2) 
                                                (at level 10, 
                                                 C1 at next level, st1 at next level, tm1 at next level,
                                                 C2 at next level, st2 at next level, tm2 at next level).
 
-Notation "'<m|' C1 st1 tm1 '~>' C2 st2 tm2 '|m>'" := (MreachM C1 st1 tm1 C2 st2 tm2) 
+Notation "'<m|' C1 st1 tm1 '~#>' C2 st2 tm2 '|m>'" := (MreachM C1 st1 tm1 C2 st2 tm2) 
                                                (at level 10, 
                                                 C1 at next level, st1 at next level, tm1 at next level,
                                                 C2 at next level, st2 at next level, tm2 at next level).
 
-Notation "'<e|' C1 st1 tm1 '~>' C2 st2 tm2 '|m>'" := (EreachM C1 st1 tm1 C2 st2 tm2) 
+Notation "'<e|' C1 st1 tm1 '~#>' C2 st2 tm2 '|m>'" := (EreachM C1 st1 tm1 C2 st2 tm2) 
                                                (at level 10, 
                                                 C1 at next level, st1 at next level, tm1 at next level,
                                                 C2 at next level, st2 at next level, tm2 at next level).
@@ -501,37 +503,37 @@ Notation "'<e|' C1 st1 tm1 '~>' C2 st2 tm2 '|m>'" := (EreachM C1 st1 tm1 C2 st2 
 Lemma ere_trans : forall C1 st1 e1
                          C2 st2 e2
                          C3 st3 e3
-                         (REACH1 : <e| C1 st1 e1 ~> C2 st2 e2 |e>)
-                         (REACH2 : <e| C2 st2 e2 ~> C3 st3 e3 |e>),
-                         <e| C1 st1 e1 ~> C3 st3 e3 |e>.
+                         (REACH1 : <e| C1 st1 e1 ~#> C2 st2 e2 |e>)
+                         (REACH2 : <e| C2 st2 e2 ~#> C3 st3 e3 |e>),
+                         <e| C1 st1 e1 ~#> C3 st3 e3 |e>.
 Proof.
   intros. generalize dependent e3.
   revert C3 st3.
   apply (_EreachE_ind_mut
     (fun C1 st1 e1 
          C2 st2 e2 
-         (REACH1 : <e| C1 st1 e1 ~> C2 st2 e2 |e>)=> 
+         (REACH1 : <e| C1 st1 e1 ~#> C2 st2 e2 |e>)=> 
          forall C3 st3 e3 
-                (REACH2 : <e| C2 st2 e2 ~> C3 st3 e3 |e>),
-                <e| C1 st1 e1 ~> C3 st3 e3 |e>)
+                (REACH2 : <e| C2 st2 e2 ~#> C3 st3 e3 |e>),
+                <e| C1 st1 e1 ~#> C3 st3 e3 |e>)
     (fun C1 st1 e1 
          C2 st2 m2 
-         (REACH1 : <e| C1 st1 e1 ~> C2 st2 m2 |m>)=> 
+         (REACH1 : <e| C1 st1 e1 ~#> C2 st2 m2 |m>)=> 
          forall C3 st3 e3 
-                (REACH2 : <m| C2 st2 m2 ~> C3 st3 e3 |e>),
-                <e| C1 st1 e1 ~> C3 st3 e3 |e>)
+                (REACH2 : <m| C2 st2 m2 ~#> C3 st3 e3 |e>),
+                <e| C1 st1 e1 ~#> C3 st3 e3 |e>)
     (fun C1 st1 m1
          C2 st2 e2
-         (REACH1 : <m| C1 st1 m1 ~> C2 st2 e2 |e>) =>
+         (REACH1 : <m| C1 st1 m1 ~#> C2 st2 e2 |e>) =>
          forall C3 st3 e3 
-                (REACH2 : <e| C2 st2 e2 ~> C3 st3 e3 |e>),
-                <m| C1 st1 m1 ~> C3 st3 e3 |e>)
+                (REACH2 : <e| C2 st2 e2 ~#> C3 st3 e3 |e>),
+                <m| C1 st1 m1 ~#> C3 st3 e3 |e>)
     (fun C1 st1 m1 
          C2 st2 m2 
-         (REACH1 : <m| C1 st1 m1 ~> C2 st2 m2 |m>)=> 
+         (REACH1 : <m| C1 st1 m1 ~#> C2 st2 m2 |m>)=> 
          forall C3 st3 e3 
-                (REACH2 : <m| C2 st2 m2 ~> C3 st3 e3 |e>),
-                <m| C1 st1 m1 ~> C3 st3 e3 |e>));
+                (REACH2 : <m| C2 st2 m2 ~#> C3 st3 e3 |e>),
+                <m| C1 st1 m1 ~#> C3 st3 e3 |e>));
    eauto using EreachE, EreachM, MreachE, MreachM;
    intros; try inversion pf; subst; inversion REACH2; subst;
    eauto using EreachE, EreachM, MreachE, MreachM.
@@ -540,37 +542,37 @@ Qed.
 Lemma mrm_trans : forall C1 st1 m1
                          C2 st2 m2
                          C3 st3 m3
-                         (REACH1 : <m| C1 st1 m1 ~> C2 st2 m2 |m>)
-                         (REACH2 : <m| C2 st2 m2 ~> C3 st3 m3 |m>),
-                         <m| C1 st1 m1 ~> C3 st3 m3 |m>.
+                         (REACH1 : <m| C1 st1 m1 ~#> C2 st2 m2 |m>)
+                         (REACH2 : <m| C2 st2 m2 ~#> C3 st3 m3 |m>),
+                         <m| C1 st1 m1 ~#> C3 st3 m3 |m>.
 Proof.
   intros. generalize dependent m3.
   revert C3 st3.
   apply (_MreachM_ind_mut
     (fun C1 st1 e1 
          C2 st2 e2 
-         (REACH1 : <e| C1 st1 e1 ~> C2 st2 e2 |e>)=> 
+         (REACH1 : <e| C1 st1 e1 ~#> C2 st2 e2 |e>)=> 
          forall C3 st3 m3 
-                (REACH2 : <e| C2 st2 e2 ~> C3 st3 m3 |m>),
-                <e| C1 st1 e1 ~> C3 st3 m3 |m>)
+                (REACH2 : <e| C2 st2 e2 ~#> C3 st3 m3 |m>),
+                <e| C1 st1 e1 ~#> C3 st3 m3 |m>)
     (fun C1 st1 e1 
          C2 st2 m2 
-         (REACH1 : <e| C1 st1 e1 ~> C2 st2 m2 |m>)=> 
+         (REACH1 : <e| C1 st1 e1 ~#> C2 st2 m2 |m>)=> 
          forall C3 st3 m3 
-                (REACH2 : <m| C2 st2 m2 ~> C3 st3 m3 |m>),
-                <e| C1 st1 e1 ~> C3 st3 m3 |m>)
+                (REACH2 : <m| C2 st2 m2 ~#> C3 st3 m3 |m>),
+                <e| C1 st1 e1 ~#> C3 st3 m3 |m>)
     (fun C1 st1 m1
          C2 st2 e2
-         (REACH1 : <m| C1 st1 m1 ~> C2 st2 e2 |e>) =>
+         (REACH1 : <m| C1 st1 m1 ~#> C2 st2 e2 |e>) =>
          forall C3 st3 m3 
-                (REACH2 : <e| C2 st2 e2 ~> C3 st3 m3 |m>),
-                <m| C1 st1 m1 ~> C3 st3 m3 |m>)
+                (REACH2 : <e| C2 st2 e2 ~#> C3 st3 m3 |m>),
+                <m| C1 st1 m1 ~#> C3 st3 m3 |m>)
     (fun C1 st1 m1 
          C2 st2 m2 
-         (REACH1 : <m| C1 st1 m1 ~> C2 st2 m2 |m>)=> 
+         (REACH1 : <m| C1 st1 m1 ~#> C2 st2 m2 |m>)=> 
          forall C3 st3 m3 
-                (REACH2 : <m| C2 st2 m2 ~> C3 st3 m3 |m>),
-                <m| C1 st1 m1 ~> C3 st3 m3 |m>));
+                (REACH2 : <m| C2 st2 m2 ~#> C3 st3 m3 |m>),
+                <m| C1 st1 m1 ~#> C3 st3 m3 |m>));
    eauto using EreachE, EreachM, MreachE, MreachM;
    intros; try inversion pf; subst; inversion REACH2; subst;
    eauto using EreachE, EreachM, MreachE, MreachM.
@@ -579,37 +581,37 @@ Qed.
 Lemma ermre_trans : forall C1 st1 e1
                            C2 st2 m2
                            C3 st3 e3
-                           (REACH1 : <e| C1 st1 e1 ~> C2 st2 m2 |m>)
-                           (REACH2 : <m| C2 st2 m2 ~> C3 st3 e3 |e>),
-                           <e| C1 st1 e1 ~> C3 st3 e3 |e>. 
+                           (REACH1 : <e| C1 st1 e1 ~#> C2 st2 m2 |m>)
+                           (REACH2 : <m| C2 st2 m2 ~#> C3 st3 e3 |e>),
+                           <e| C1 st1 e1 ~#> C3 st3 e3 |e>. 
 Proof.
   intros. generalize dependent e3.
   revert C3 st3.
   apply (_EreachM_ind_mut
     (fun C1 st1 e1 
          C2 st2 e2 
-         (REACH1 : <e| C1 st1 e1 ~> C2 st2 e2 |e>)=> 
+         (REACH1 : <e| C1 st1 e1 ~#> C2 st2 e2 |e>)=> 
          forall C3 st3 e3 
-                (REACH2 : <e| C2 st2 e2 ~> C3 st3 e3 |e>),
-                <e| C1 st1 e1 ~> C3 st3 e3 |e>)
+                (REACH2 : <e| C2 st2 e2 ~#> C3 st3 e3 |e>),
+                <e| C1 st1 e1 ~#> C3 st3 e3 |e>)
     (fun C1 st1 e1 
          C2 st2 m2 
-         (REACH1 : <e| C1 st1 e1 ~> C2 st2 m2 |m>)=> 
+         (REACH1 : <e| C1 st1 e1 ~#> C2 st2 m2 |m>)=> 
          forall C3 st3 e3 
-                (REACH2 : <m| C2 st2 m2 ~> C3 st3 e3 |e>),
-                <e| C1 st1 e1 ~> C3 st3 e3 |e>)
+                (REACH2 : <m| C2 st2 m2 ~#> C3 st3 e3 |e>),
+                <e| C1 st1 e1 ~#> C3 st3 e3 |e>)
     (fun C1 st1 m1
          C2 st2 e2
-         (REACH1 : <m| C1 st1 m1 ~> C2 st2 e2 |e>) =>
+         (REACH1 : <m| C1 st1 m1 ~#> C2 st2 e2 |e>) =>
          forall C3 st3 e3 
-                (REACH2 : <e| C2 st2 e2 ~> C3 st3 e3 |e>),
-                <m| C1 st1 m1 ~> C3 st3 e3 |e>)
+                (REACH2 : <e| C2 st2 e2 ~#> C3 st3 e3 |e>),
+                <m| C1 st1 m1 ~#> C3 st3 e3 |e>)
     (fun C1 st1 m1 
          C2 st2 m2 
-         (REACH1 : <m| C1 st1 m1 ~> C2 st2 m2 |m>)=> 
+         (REACH1 : <m| C1 st1 m1 ~#> C2 st2 m2 |m>)=> 
          forall C3 st3 e3 
-                (REACH2 : <m| C2 st2 m2 ~> C3 st3 e3 |e>),
-                <m| C1 st1 m1 ~> C3 st3 e3 |e>));
+                (REACH2 : <m| C2 st2 m2 ~#> C3 st3 e3 |e>),
+                <m| C1 st1 m1 ~#> C3 st3 e3 |e>));
    eauto using EreachE, EreachM, MreachE, MreachM;
    intros; try inversion pf; subst; inversion REACH2; subst;
    eauto using EreachE, EreachM, MreachE, MreachM.
@@ -618,43 +620,43 @@ Qed.
 Lemma mrerm_trans : forall C1 st1 m1
                            C2 st2 e2
                            C3 st3 m3
-                           (REACH1 : <m| C1 st1 m1 ~> C2 st2 e2 |e>)
-                           (REACH2 : <e| C2 st2 e2 ~> C3 st3 m3 |m>),
-                           <m| C1 st1 m1 ~> C3 st3 m3 |m>. 
+                           (REACH1 : <m| C1 st1 m1 ~#> C2 st2 e2 |e>)
+                           (REACH2 : <e| C2 st2 e2 ~#> C3 st3 m3 |m>),
+                           <m| C1 st1 m1 ~#> C3 st3 m3 |m>. 
 Proof.
   intros. generalize dependent m3.
   revert C3 st3.
   apply (_MreachE_ind_mut
     (fun C1 st1 e1 
          C2 st2 e2 
-         (REACH1 : <e| C1 st1 e1 ~> C2 st2 e2 |e>)=> 
+         (REACH1 : <e| C1 st1 e1 ~#> C2 st2 e2 |e>)=> 
          forall C3 st3 m3 
-                (REACH2 : <e| C2 st2 e2 ~> C3 st3 m3 |m>),
-                <e| C1 st1 e1 ~> C3 st3 m3 |m>)
+                (REACH2 : <e| C2 st2 e2 ~#> C3 st3 m3 |m>),
+                <e| C1 st1 e1 ~#> C3 st3 m3 |m>)
     (fun C1 st1 e1 
          C2 st2 m2 
-         (REACH1 : <e| C1 st1 e1 ~> C2 st2 m2 |m>)=> 
+         (REACH1 : <e| C1 st1 e1 ~#> C2 st2 m2 |m>)=> 
          forall C3 st3 m3 
-                (REACH2 : <m| C2 st2 m2 ~> C3 st3 m3 |m>),
-                <e| C1 st1 e1 ~> C3 st3 m3 |m>)
+                (REACH2 : <m| C2 st2 m2 ~#> C3 st3 m3 |m>),
+                <e| C1 st1 e1 ~#> C3 st3 m3 |m>)
     (fun C1 st1 m1
          C2 st2 e2
-         (REACH1 : <m| C1 st1 m1 ~> C2 st2 e2 |e>) =>
+         (REACH1 : <m| C1 st1 m1 ~#> C2 st2 e2 |e>) =>
          forall C3 st3 m3 
-                (REACH2 : <e| C2 st2 e2 ~> C3 st3 m3 |m>),
-                <m| C1 st1 m1 ~> C3 st3 m3 |m>)
+                (REACH2 : <e| C2 st2 e2 ~#> C3 st3 m3 |m>),
+                <m| C1 st1 m1 ~#> C3 st3 m3 |m>)
     (fun C1 st1 m1 
          C2 st2 m2 
-         (REACH1 : <m| C1 st1 m1 ~> C2 st2 m2 |m>)=> 
+         (REACH1 : <m| C1 st1 m1 ~#> C2 st2 m2 |m>)=> 
          forall C3 st3 m3 
-                (REACH2 : <m| C2 st2 m2 ~> C3 st3 m3 |m>),
-                <m| C1 st1 m1 ~> C3 st3 m3 |m>));
+                (REACH2 : <m| C2 st2 m2 ~#> C3 st3 m3 |m>),
+                <m| C1 st1 m1 ~#> C3 st3 m3 |m>));
    eauto using EreachE, EreachM, MreachE, MreachM;
    intros; try inversion pf; subst; inversion REACH2; subst;
    eauto using EreachE, EreachM, MreachE, MreachM.
 Qed.
 
-Lemma c_plugin_assoc : forall C1 C2 C3, C1[| C2[| C3 |] |] = ((C1[|C2|])[|C3|]).
+Lemma c_plugin_assoc : forall C1 C2 C3, C1[#| C2[#| C3 |#] |#] = ((C1[#|C2|#])[#|C3|#]).
 Proof.
   induction C1; eauto; 
   intros; simpl; try rewrite IHC1; eauto.
@@ -670,10 +672,10 @@ Proof.
   - split; eauto.
   - split; intros contra; inversion contra.
   - split; intros contra; inversion contra.
-  - unfold eq_t. remember (a =? a0) as eqa.
-    destruct eqa; simpl; symmetry in Heqeqa;
-    try rewrite Nat.eqb_eq in Heqeqa;
-    try rewrite Nat.eqb_neq in Heqeqa.
+  - simpl. remember (eq_t a a0) as eqa.
+    destruct eqa; symmetry in Heqeqa;
+    try rewrite eq_t_eq in Heqeqa;
+    try rewrite eq_t_neq in Heqeqa.
     + split; intros. rewrite Heqeqa in *.
       apply IHp1 in H. rewrite H. eauto.
       eapply IHp1. inversion H; eauto.
@@ -681,19 +683,24 @@ Proof.
       apply Heqeqa in H0; inversion H0.
 Qed.
 
-Lemma c_plugin_adds_level : forall C1 C2, eq_p (dy_level(C1[|C2|])) (dy_level C1 ++ dy_level C2) = true.
+Lemma c_plugin_adds_level : forall C1 C2, eq_p (dy_level(C1[#|C2|#])) (dy_level C1 ++ dy_level C2) = true.
 Proof.
   induction C1; induction C2;
   intros; simpl; 
-  try rewrite IHC1; try rewrite IHC2; try unfold eq_t;
-  eauto; try (assert (RR : tx =? tx = true);
-  try apply Nat.eqb_eq; eauto; try rewrite RR; try clear RR; eauto).
-  - assert (RR : dy_level (dy_c_letm M C2_1 C2_2) = dy_level C2_2); eauto;
-    rewrite <- RR; clear RR; eapply IHC1.
-  - assert (RR : dy_level (dy_c_letm M C2_1 C2_2) = dy_level C2_2); eauto;
-    rewrite <- RR; clear RR; eapply IHC1.
-  - assert (RR : dy_level (dy_c_letm M0 C2_1 C2_2) = dy_level C2_2); eauto;
-    rewrite <- RR; clear RR; eapply IHC1_2.
+  try rewrite IHC1; try rewrite IHC2;
+  eauto; try (assert (RR : eq_t tx tx = true);
+  try apply eq_t_eq; eauto; try rewrite RR; try clear RR; eauto).
+  - simpl in *. rewrite IHC2. eauto.
+  - simpl in *. rewrite IHC2. eauto.
+  - assert (RR : forall C2, dy_level (dy_c_letm M C2_1 C2) = dy_level C2); eauto.
+    specialize (IHC1 (dy_c_letm M C2_1 C2_2)).
+    rewrite RR in IHC1. rewrite IHC1. eauto.
+  - assert (RR : forall C2, dy_level (dy_c_letm M C2_1 C2) = dy_level C2); eauto.
+    specialize (IHC1 (dy_c_letm M C2_1 C2_2)).
+    rewrite RR in IHC1. rewrite IHC1. eauto.
+  - assert (RR : forall C2, dy_level (dy_c_letm M0 C2_1 C2) = dy_level C2); eauto.
+    specialize (IHC1_2 (dy_c_letm M0 C2_1 C2_2)).
+    rewrite RR in IHC1_2. rewrite IHC1_2. eauto.
 Qed.
 
 (* equivalence between reachability relations *)
@@ -703,7 +710,7 @@ Lemma Eeval_then_reach :
            ev pf Cv mem t
            (VAL : v = Val ev pf Cv)
            (STATE : stv = ST mem t),
-          <e| Ci sti ei ~> Cv stv ev |e>.
+          <e| Ci sti ei ~#> Cv stv ev |e>.
 Proof.
   apply (EevalR_ind_mut
     (fun Ci sti ei v stv
@@ -711,10 +718,10 @@ Proof.
         forall ev pf Cv mem t
               (VAL : v = Val ev pf Cv)
               (STATE : stv = ST mem t),
-        <e| Ci sti ei ~> Cv stv ev |e>)
+        <e| Ci sti ei ~#> Cv stv ev |e>)
     (fun Ci sti mi Cv stv
         (EVAL : MevalR Ci sti mi Cv stv) =>
-        <m| Ci sti mi ~> Cv stv m_empty |m>));
+        <m| Ci sti mi ~#> Cv stv m_empty |m>));
   intros; try inversion STATE0; try inversion STATE;
           try inversion VAL; try destruct st_lam;
           try destruct st_m; try destruct v_e;
@@ -725,7 +732,7 @@ Qed.
 Lemma Meval_then_reach :
     forall Ci sti mi Cv stv
            (EVAL : MevalR Ci sti mi Cv stv),
-           <m| Ci sti mi ~> Cv stv m_empty |m>.
+           <m| Ci sti mi ~#> Cv stv m_empty |m>.
 Proof.
   apply (MevalR_ind_mut
     (fun Ci sti ei v stv
@@ -733,10 +740,10 @@ Proof.
         forall ev pf Cv mem t
               (VAL : v = Val ev pf Cv)
               (STATE : stv = ST mem t),
-        <e| Ci sti ei ~> Cv stv ev |e>)
+        <e| Ci sti ei ~#> Cv stv ev |e>)
     (fun Ci sti mi Cv stv
         (EVAL : MevalR Ci sti mi Cv stv) =>
-        <m| Ci sti mi ~> Cv stv m_empty |m>));
+        <m| Ci sti mi ~#> Cv stv m_empty |m>));
   intros; try inversion STATE0; try inversion STATE;
           try inversion VAL; try destruct st_lam;
           try destruct st_m; try destruct v_e;
@@ -746,21 +753,21 @@ Qed.
 
 Lemma EreachE_equiv_left :
     forall C1 st1 e1 C2 st2 e2,
-          <e| C1 st1 e1 ~> C2 st2 e2 |e> ->
+          <e| C1 st1 e1 ~#> C2 st2 e2 |e> ->
           _EreachE C1 st1 e1 C2 st2 e2.
 Proof.
   apply (_EreachE_ind_mut 
     (fun C1 st1 e1 C2 st2 e2
-        (REACH : <e| C1 st1 e1 ~> C2 st2 e2 |e>) =>
+        (REACH : <e| C1 st1 e1 ~#> C2 st2 e2 |e>) =>
         _EreachE C1 st1 e1 C2 st2 e2)
     (fun C1 st1 e1 C2 st2 m2
-        (REACH : <e| C1 st1 e1 ~> C2 st2 m2 |m>) =>
+        (REACH : <e| C1 st1 e1 ~#> C2 st2 m2 |m>) =>
         _EreachM C1 st1 e1 C2 st2 m2)
     (fun C1 st1 m1 C2 st2 e2
-        (REACH : <m| C1 st1 m1 ~> C2 st2 e2 |e>) =>
+        (REACH : <m| C1 st1 m1 ~#> C2 st2 e2 |e>) =>
         _MreachE C1 st1 m1 C2 st2 e2)
     (fun C1 st1 m1 C2 st2 m2
-        (REACH : <m| C1 st1 m1 ~> C2 st2 m2 |m>) =>
+        (REACH : <m| C1 st1 m1 ~#> C2 st2 m2 |m>) =>
         _MreachM C1 st1 m1 C2 st2 m2));
   intros; eauto using EreachE, EreachM, MreachE, MreachM, _EreachE, _MreachE, _EreachM, _MreachM.
 Qed.
@@ -768,15 +775,15 @@ Qed.
 Lemma EreachE_equiv_right :
     forall C1 st1 e1 C2 st2 e2,
           _EreachE C1 st1 e1 C2 st2 e2 ->
-          <e| C1 st1 e1 ~> C2 st2 e2 |e>.
+          <e| C1 st1 e1 ~#> C2 st2 e2 |e>.
 Proof.
   apply (__EreachE_ind_mut 
     (fun C1 st1 e1 C2 st2 e2
         (REACH : _EreachE C1 st1 e1 C2 st2 e2) =>
-        <e| C1 st1 e1 ~> C2 st2 e2 |e>)
+        <e| C1 st1 e1 ~#> C2 st2 e2 |e>)
     (fun C1 st1 m1 C2 st2 e2
         (REACH : _MreachE C1 st1 m1 C2 st2 e2) =>
-        <m| C1 st1 m1 ~> C2 st2 e2 |e>));
+        <m| C1 st1 m1 ~#> C2 st2 e2 |e>));
   intros; try destruct v; try destruct st; try destruct st1; try destruct st_lam;
   try destruct arg; try destruct st_m; try destruct st';
   eauto using EreachE, EreachM, MreachE, MreachM, _EreachE, _MreachE, _EreachM, _MreachM.
@@ -791,73 +798,14 @@ Qed.
 Theorem EreachE_equiv : 
   forall C1 st1 e1 C2 st2 e2,
          _EreachE C1 st1 e1 C2 st2 e2 <->
-          <e| C1 st1 e1 ~> C2 st2 e2 |e>.
+          <e| C1 st1 e1 ~#> C2 st2 e2 |e>.
 Proof. 
   intros; split; try apply EreachE_equiv_left; try apply EreachE_equiv_right. 
 Qed.
 
-Inductive st_ctx :=
-  | st_c_hole
-  | st_c_lam (x : expr_id) (C : st_ctx)
-  | st_c_lete (x : expr_id) (C : st_ctx)
-  | st_c_letm (M : mod_id) (CM : st_ctx) (C : st_ctx)
-.
-
-Fixpoint st_level (C : st_ctx) : nat :=
-  match C with
-  | st_c_hole => 0
-  | st_c_lam _ C'
-  | st_c_lete _ C' => S (st_level C')
-  | st_c_letm _ _ C' => st_level C'
-  end.
-
-Fixpoint st_ctx_M (C : st_ctx) (M : mod_id) :=
-  match C with
-  | st_c_hole => None
-  | st_c_lam _ C'
-  | st_c_lete _ C' => st_ctx_M C' M
-  | st_c_letm M' CM' C' =>
-    match st_ctx_M C' M with
-    | Some CM => Some CM
-    | None => if eq_mid M M' then Some CM' else None
-    end
-  end.
-
-Fixpoint st_c_plugin (Cout : st_ctx) (Cin : st_ctx) :=
-  match Cout with
-  | st_c_hole => Cin
-  | st_c_lam x C' => st_c_lam x (st_c_plugin C' Cin)
-  | st_c_lete x C' => st_c_lete x (st_c_plugin C' Cin)
-  | st_c_letm M' CM' C' => st_c_letm M' CM' (st_c_plugin C' Cin)
-  end.
-
-Lemma st_c_plugin_assoc : forall C1 C2 C3,
-  st_c_plugin (st_c_plugin C1 C2) C3 =
-  st_c_plugin C1 (st_c_plugin C2 C3). 
-Proof.
-  induction C1; eauto; 
-  intros; simpl; try rewrite IHC1; eauto.
-  rewrite IHC1_2. eauto.
-Qed.
-
-Lemma st_c_plugin_add_level :
-  forall C1 C2, st_level (st_c_plugin C1 C2) = st_level C1 + st_level C2.
-Proof.
-  induction C1; induction C2; intros; simpl; eauto.
-  - assert (RR : st_level (st_c_letm M C2_1 C2_2) = st_level C2_2); eauto.
-    specialize (IHC1 (st_c_letm M C2_1 C2_2)).
-    rewrite IHC1. rewrite RR. eauto.
-  - assert (RR : st_level (st_c_letm M C2_1 C2_2) = st_level C2_2); eauto.
-    specialize (IHC1 (st_c_letm M C2_1 C2_2)).
-    rewrite IHC1. rewrite RR. eauto.
-  - assert (RR : st_level (st_c_letm M0 C2_1 C2_2) = st_level C2_2); eauto.
-    specialize (IHC1_2 (st_c_letm M0 C2_1 C2_2)).
-    rewrite IHC1_2. rewrite RR. eauto.
-Qed.
-
 Fixpoint dy_to_st C :=
   match C with
-  |  ([||]) => st_c_hole
+  |  ([#||#]) => st_c_hole
   | dy_c_lam x _ C' => st_c_lam x (dy_to_st C')
   | dy_c_lete x _ C' => st_c_lete x (dy_to_st C')
   | dy_c_letm M CM C' => st_c_letm M (dy_to_st CM) (dy_to_st C')
@@ -865,7 +813,7 @@ Fixpoint dy_to_st C :=
 
 Lemma dy_to_st_plugin :
   forall Cout Cin,
-    dy_to_st (Cout[|Cin|]) = st_c_plugin (dy_to_st Cout) (dy_to_st Cin).
+    dy_to_st (Cout[#|Cin|#]) = st_c_plugin (dy_to_st Cout) (dy_to_st Cin).
 Proof.
   induction Cout; intros; simpl; try rewrite IHCout; eauto.
   rewrite IHCout2. eauto.
@@ -964,8 +912,8 @@ Lemma EreachE_ind_mut :
             Pe C st (e_app e1 e2) ->
             Pe C_lam st_lam (e_lam x e) ->
             Pe C_arg (ST mem t) arg ->
-            Pe (C_lam[|dy_c_lam x t ([||])|])
-              (ST ((dy_level C_lam ++ [t]) !-> (Val arg pf C_arg) ; mem) (update_t t)) e) ->
+            Pe (C_lam[#|dy_c_lam x t ([#||#])|#])
+              (ST ((dy_level C_lam ++ [t]) !#-> (Val arg pf C_arg) ; mem) (update_t t)) e) ->
     (forall C st m e, Pe C st (e_link m e) -> Pm C st m) ->
     (forall C st m e C_m st_m,
             Pe C st (e_link m e) -> (MevalR C st m C_m st_m) ->
@@ -977,18 +925,18 @@ Lemma EreachE_ind_mut :
     (forall C st x e m C_x mem t v pf,
             Pm C st (m_lete x e m) ->
             Pe C_x (ST mem t) v ->
-            Pm (C[|dy_c_lete x t  ([||])|])
-              (ST ((dy_level C ++ [t]) !-> (Val v pf C_x) ; mem) (update_t t)) m) ->
+            Pm (C[#|dy_c_lete x t  ([#||#])|#])
+              (ST ((dy_level C ++ [t]) !#-> (Val v pf C_x) ; mem) (update_t t)) m) ->
     (forall C st M m1 m2,
             Pm C st (m_letm M m1 m2) -> Pm C st m1) ->
     (forall C st M m1 m2 C_M st_M,
             Pm C st (m_letm M m1 m2) ->
             (MevalR C st m1 C_M st_M) ->
             Pm C_M st_M m_empty ->
-            Pm (C[|dy_c_letm M C_M  ([||])|]) st_M m2) ->
+            Pm (C[#|dy_c_letm M C_M  ([#||#])|#]) st_M m2) ->
     (forall C st e C' st' e'
             (INIT : Pe C st e)
-            (REACH : <e| C st e ~> C' st' e' |e>),
+            (REACH : <e| C st e ~#> C' st' e' |e>),
             Pe C' st' e').
 Proof. 
 (* intros just before our goal, then fix 8, on REACH, 
@@ -997,17 +945,17 @@ Proof.
   fix IHere 8 with 
     (IHerm C st e C' st' m'
           (INIT : Pe C st e)
-          (REACH : <e| C st e ~> C' st' m' |m>)
+          (REACH : <e| C st e ~#> C' st' m' |m>)
           { struct REACH }
           : Pm C' st' m')
     (IHmre C st m C' st' e'
           (INIT : Pm C st m)
-          (REACH : <m| C st m ~> C' st' e' |e>)
+          (REACH : <m| C st m ~#> C' st' e' |e>)
           { struct REACH }
           : Pe C' st' e')
     (IHmrm C st m C' st' m'
           (INIT : Pm C st m)
-          (REACH : <m| C st m ~> C' st' m' |m>)
+          (REACH : <m| C st m ~#> C' st' m' |m>)
           { struct REACH }
           : Pm C' st' m').
   - intros. destruct REACH.
@@ -1025,8 +973,8 @@ Proof.
     + assert (LAM : Pe C_lam st_lam (e_lam x e)).
       apply (IHere C st e1 C_lam st_lam (e_lam x e)).
       eapply APPl. exact INIT. exact REACH1.
-      apply (IHere (C_lam [|dy_c_lam x t ([||])|])
-            (ST (dy_level C_lam ++ [t] !-> Val arg pf C_arg; mem)
+      apply (IHere (C_lam [#|dy_c_lam x t ([#||#])|#])
+            (ST (dy_level C_lam ++ [t] !#-> Val arg pf C_arg; mem)
             (update_t t)) e C' st' e').
       apply APPb with (C := C) (st := st) (e1 := e1) (e2 := e2) (st_lam := st_lam).
       exact INIT. exact LAM. 
@@ -1048,8 +996,8 @@ Proof.
     + assert (LAM : Pe C_lam st_lam (e_lam x e)).
       apply (IHere C st e1 C_lam st_lam (e_lam x e)).
       eapply APPl. exact INIT. exact FNr.
-      apply (IHerm (C_lam [|dy_c_lam x t ([||])|])
-            (ST (dy_level C_lam ++ [t] !-> Val arg pf C_arg; mem)
+      apply (IHerm (C_lam [#|dy_c_lam x t ([#||#])|#])
+            (ST (dy_level C_lam ++ [t] !#-> Val arg pf C_arg; mem)
             (update_t t)) e C' st' m').
       eapply APPb with (st_lam := st_lam). exact INIT. exact LAM.
       apply (IHere C st_lam e2 C_arg (ST mem t) arg).
@@ -1064,15 +1012,15 @@ Proof.
   - intros. destruct REACH.
     + apply (IHere C st e C' st' e').
       eapply LETex. exact INIT. exact REACHe.
-    + apply (IHmre (C [|dy_c_lete x t ([||])|])
-        (ST (dy_level C ++ [t] !-> Val v pf C_x; mem) (update_t t)) m
+    + apply (IHmre (C [#|dy_c_lete x t ([#||#])|#])
+        (ST (dy_level C ++ [t] !#-> Val v pf C_x; mem) (update_t t)) m
         C' st' e').
       eapply LETem. exact INIT.
       apply (IHere C st e C_x (ST mem t) v).
       eapply LETex. exact INIT. exact EVALxr. exact REACH.
     + apply (IHmre C st m1 C' st' e').
       eapply LETm1. exact INIT. exact REACH.
-    + apply (IHmre (C [|dy_c_letm M C_M ([||])|]) st_M m2 C' st' e').
+    + apply (IHmre (C [#|dy_c_letm M C_M ([#||#])|#]) st_M m2 C' st' e').
       eapply LETm2. exact INIT. exact EVALM.
       apply (IHmrm C st m1 C_M st_M m_empty).
       eapply LETm1. exact INIT. exact EVALM0. exact REACH.
@@ -1082,15 +1030,15 @@ Proof.
       apply MVAR. exact INIT.
     + apply (IHerm C st e C' st' m').
       eapply LETex. exact INIT. exact REACHe.
-    + apply (IHmrm (C [|dy_c_lete x t ([||])|])
-        (ST (dy_level C ++ [t] !-> Val v pf C_x; mem) (update_t t)) m
+    + apply (IHmrm (C [#|dy_c_lete x t ([#||#])|#])
+        (ST (dy_level C ++ [t] !#-> Val v pf C_x; mem) (update_t t)) m
         C' st' m').
       eapply LETem. exact INIT.
       apply (IHere C st e C_x (ST mem t) v).
       eapply LETex. exact INIT. exact EVALxr. exact REACH.
     + apply (IHmrm C st m1 C' st' m').
       eapply LETm1. exact INIT. exact REACH.
-    + apply (IHmrm (C [|dy_c_letm M C_M ([||])|]) st_M m2 C' st' m').
+    + apply (IHmrm (C [#|dy_c_letm M C_M ([#||#])|#]) st_M m2 C' st' m').
       eapply LETm2. exact INIT. exact EVALM.
       apply (IHmrm C st m1 C_M st_M m_empty).
       eapply LETm1. exact INIT. exact REACH1. exact REACH2.
@@ -1099,7 +1047,7 @@ Qed.
 Lemma value_reach_only_itself_e :
   forall C st v (pf : value v)
          C' st' e'
-         (REACH : <e| C st v ~> C' st' e' |e>),
+         (REACH : <e| C st v ~#> C' st' e' |e>),
          C = C' /\ st = st' /\ v = e'.
 Proof.
   intros; repeat split; inversion pf; inversion REACH; subst; eauto using EreachE;
@@ -1109,66 +1057,12 @@ Qed.
 Lemma value_reach_only_itself_m :
   forall C st v (pf : value v)
          C' st' m'
-         (REACH : <e| C st v ~> C' st' m' |m>),
+         (REACH : <e| C st v ~#> C' st' m' |m>),
          False.
 Proof.
   intros; repeat split; inversion pf; inversion REACH; subst; eauto using EreachM;
   try inversion H0.
 Qed.
-
-Notation "Cout '[[|' Cin '|]]'" := (st_c_plugin Cout Cin)
-                              (at level 100, Cin at next level, right associativity).
-
-Notation "'[[||]]'" := (st_c_hole) (at level 100).
-
-(* collect all static contexts reachable from the current configuration *)
-Fixpoint collect_ctx_expr C e :=
-  match e with
-  | e_var x => [C]
-  | e_lam x e' => C :: collect_ctx_expr
-                       (C [[|st_c_lam x ([[||]]) |]]) e'
-  | e_app e1 e2 =>
-    let ctxs1 := collect_ctx_expr C e1 in
-    let ctxs2 := collect_ctx_expr C e2 in
-    ctxs1 ++ ctxs2
-  | e_link m e' =>
-    match collect_ctx_mod C m with
-    | (Some C_m, ctxs_m) => 
-      let ctxs_e := collect_ctx_expr C_m e' in
-      ctxs_m ++ ctxs_e
-    | (None, ctxs_m) => ctxs_m
-    end
-  end
-
-with collect_ctx_mod C m :=
-  match m with
-  | m_empty => (Some C, [C])
-  | m_var M =>
-    match st_ctx_M C M with
-    | Some C_M => (Some C_M, [C ; C_M])
-    | None => (None, [C])
-    end
-  | m_lete x e m' =>
-    let ctxs_e := collect_ctx_expr C e in
-    let (ctx_o, ctxs_m) := collect_ctx_mod 
-                           (C [[| st_c_lete x ([[||]]) |]]) m' in
-    (ctx_o, ctxs_e ++ ctxs_m)
-  | m_letm M m1 m2 =>
-    match collect_ctx_mod C m1 with
-    | (Some C_M, ctxs_m1) => 
-      let (ctx_o, ctxs_m2) := collect_ctx_mod
-                              (C [[| st_c_letm M C_M ([[||]]) |]]) m2 in
-      (ctx_o, ctxs_m1 ++ ctxs_m2)
-    | (None, ctxs_m1) => (None, ctxs_m1)
-    end
-  end.
-
-Compute collect_ctx_expr ([[||]]) (e_app (e_lam (eid 0) (e_var (eid 0)))
-                                  (e_lam (eid 0) (e_var (eid 0)))).
-
-Search In _ (_ ++ _).
-Search In _ (_ :: _).
-Print In.
 
 Lemma collect_ctx_expr_refl : forall e C, In C (collect_ctx_expr C e).
 Proof.
@@ -1246,7 +1140,7 @@ Lemma ere_ctx_bound :
          C st e
          C' st' e'
          (INIT : ctx_bound_expr ub C st e)
-         (REACH : <e| C st e ~> C' st' e' |e>),
+         (REACH : <e| C st e ~#> C' st' e' |e>),
     ctx_bound_expr ub C' st' e'.
 Proof.
   intros ub.
@@ -1350,13 +1244,13 @@ Qed.
 
 Theorem expr_ctx_bound :
   forall e C' st' e'
-         (REACH : <e|  ([||]) (ST empty_mem 0) e ~> C' st' e' |e>),
+         (REACH : <e| ([#||#]) (ST empty_mem true) e ~#> C' st' e' |e>),
          In (dy_to_st C') (collect_ctx_expr ([[||]]) e).
 Proof.
   intros.
-  pose proof (ere_ctx_bound (collect_ctx_expr st_c_hole e)  ([||]) (ST empty_mem 0) e C' st' e') as H.
-  assert (ctx_bound_expr (collect_ctx_expr ([[||]]) e)  ([||])
-          (ST empty_mem 0) e) as FINAL.
+  pose proof (ere_ctx_bound (collect_ctx_expr st_c_hole e) ([#||#]) (ST empty_mem true) e C' st' e') as H.
+  assert (ctx_bound_expr (collect_ctx_expr ([[||]]) e) ([#||#])
+          (ST empty_mem true) e) as FINAL.
   - unfold ctx_bound_expr; split; simpl; eauto.
   - apply H in FINAL; try apply REACH. 
     destruct FINAL as [MEM KILLER].
