doc/coq/Concrete.v
@@ -1,4 +1,4 @@
-Require Export Modular.Syntax.
+From MODULAR Require Export Syntax.
 
 Definition time := nat.
 
@@ -33,16 +33,6 @@ Fixpoint dy_plugin_c Cout Cin :=
   | dy_c_lam x tx C' => dy_c_lam x tx (dy_plugin_c C' Cin)
   | dy_c_lete x tx C' => dy_c_lete x tx (dy_plugin_c C' Cin)
   | dy_c_letm M CM C' => dy_c_letm M CM (dy_plugin_c C' Cin)
-  end.
-
-Definition eq_eid id1 id2 :=
-  match id1, id2 with
-  | eid x1, eid x2 => x1 =? x2
-  end.
-
-Definition eq_mid id1 id2 :=
-  match id1, id2 with
-  | mid M1, mid M2 => M1 =? M2
   end.
 
 Fixpoint dy_level (C : dy_ctx) : path :=
@@ -259,7 +249,7 @@ Inductive _MreachM (C : dy_ctx) (st : state)
   | _mrm_letm_m2 M m1 m2 C_M st_M
                  C' st' m'
              (EVALM : MevalR C st m1 C_M st_M)
-             (REACHm : _MreachM (C[|dy_c_letm M C_M  ([||])|]) st_M m2
+             (REACHm : _MreachM (C[|dy_c_letm M C_M ([||])|]) st_M m2
                                  C' st' m')
     : _MreachM C st (m_letm M m1 m2)
                C' st' m'
@@ -787,68 +777,9 @@ Proof.
   intros; split; try apply EreachE_equiv_left; try apply EreachE_equiv_right. 
 Qed.
 
-Inductive st_ctx :=
-  | st_c_hole
-  | st_c_lam (x : expr_id) (C : st_ctx)
-  | st_c_lete (x : expr_id) (C : st_ctx)
-  | st_c_letm (M : mod_id) (CM : st_ctx) (C : st_ctx)
-.
-
-Fixpoint st_level (C : st_ctx) : nat :=
-  match C with
-  | st_c_hole => 0
-  | st_c_lam _ C'
-  | st_c_lete _ C' => S (st_level C')
-  | st_c_letm _ _ C' => st_level C'
-  end.
-
-Fixpoint st_ctx_M (C : st_ctx) (M : mod_id) :=
-  match C with
-  | st_c_hole => None
-  | st_c_lam _ C'
-  | st_c_lete _ C' => st_ctx_M C' M
-  | st_c_letm M' CM' C' =>
-    match st_ctx_M C' M with
-    | Some CM => Some CM
-    | None => if eq_mid M M' then Some CM' else None
-    end
-  end.
-
-Fixpoint st_c_plugin (Cout : st_ctx) (Cin : st_ctx) :=
-  match Cout with
-  | st_c_hole => Cin
-  | st_c_lam x C' => st_c_lam x (st_c_plugin C' Cin)
-  | st_c_lete x C' => st_c_lete x (st_c_plugin C' Cin)
-  | st_c_letm M' CM' C' => st_c_letm M' CM' (st_c_plugin C' Cin)
-  end.
-
-Lemma st_c_plugin_assoc : forall C1 C2 C3,
-  st_c_plugin (st_c_plugin C1 C2) C3 =
-  st_c_plugin C1 (st_c_plugin C2 C3). 
-Proof.
-  induction C1; eauto; 
-  intros; simpl; try rewrite IHC1; eauto.
-  rewrite IHC1_2. eauto.
-Qed.
-
-Lemma st_c_plugin_add_level :
-  forall C1 C2, st_level (st_c_plugin C1 C2) = st_level C1 + st_level C2.
-Proof.
-  induction C1; induction C2; intros; simpl; eauto.
-  - assert (RR : st_level (st_c_letm M C2_1 C2_2) = st_level C2_2); eauto.
-    specialize (IHC1 (st_c_letm M C2_1 C2_2)).
-    rewrite IHC1. rewrite RR. eauto.
-  - assert (RR : st_level (st_c_letm M C2_1 C2_2) = st_level C2_2); eauto.
-    specialize (IHC1 (st_c_letm M C2_1 C2_2)).
-    rewrite IHC1. rewrite RR. eauto.
-  - assert (RR : st_level (st_c_letm M0 C2_1 C2_2) = st_level C2_2); eauto.
-    specialize (IHC1_2 (st_c_letm M0 C2_1 C2_2)).
-    rewrite IHC1_2. rewrite RR. eauto.
-Qed.
-
 Fixpoint dy_to_st C :=
   match C with
-  |  ([||]) => st_c_hole
+  | ([||]) => st_c_hole
   | dy_c_lam x _ C' => st_c_lam x (dy_to_st C')
   | dy_c_lete x _ C' => st_c_lete x (dy_to_st C')
   | dy_c_letm M CM C' => st_c_letm M (dy_to_st CM) (dy_to_st C')
@@ -1104,60 +1035,6 @@ Proof.
   intros; repeat split; inversion pf; inversion REACH; subst; eauto using EreachM;
   try inversion H0.
 Qed.
-
-Notation "Cout '[[|' Cin '|]]'" := (st_c_plugin Cout Cin)
-                              (at level 100, Cin at next level, right associativity).
-
-Notation "'[[||]]'" := (st_c_hole) (at level 100).
-
-(* collect all static contexts reachable from the current configuration *)
-Fixpoint collect_ctx_expr C e :=
-  match e with
-  | e_var x => [C]
-  | e_lam x e' => C :: collect_ctx_expr
-                       (C [[|st_c_lam x ([[||]]) |]]) e'
-  | e_app e1 e2 =>
-    let ctxs1 := collect_ctx_expr C e1 in
-    let ctxs2 := collect_ctx_expr C e2 in
-    ctxs1 ++ ctxs2
-  | e_link m e' =>
-    match collect_ctx_mod C m with
-    | (Some C_m, ctxs_m) => 
-      let ctxs_e := collect_ctx_expr C_m e' in
-      ctxs_m ++ ctxs_e
-    | (None, ctxs_m) => ctxs_m
-    end
-  end
-
-with collect_ctx_mod C m :=
-  match m with
-  | m_empty => (Some C, [C])
-  | m_var M =>
-    match st_ctx_M C M with
-    | Some C_M => (Some C_M, [C ; C_M])
-    | None => (None, [C])
-    end
-  | m_lete x e m' =>
-    let ctxs_e := collect_ctx_expr C e in
-    let (ctx_o, ctxs_m) := collect_ctx_mod 
-                           (C [[| st_c_lete x ([[||]]) |]]) m' in
-    (ctx_o, ctxs_e ++ ctxs_m)
-  | m_letm M m1 m2 =>
-    match collect_ctx_mod C m1 with
-    | (Some C_M, ctxs_m1) => 
-      let (ctx_o, ctxs_m2) := collect_ctx_mod
-                              (C [[| st_c_letm M C_M ([[||]]) |]]) m2 in
-      (ctx_o, ctxs_m1 ++ ctxs_m2)
-    | (None, ctxs_m1) => (None, ctxs_m1)
-    end
-  end.
-
-Compute collect_ctx_expr ([[||]]) (e_app (e_lam (eid 0) (e_var (eid 0)))
-                                  (e_lam (eid 0) (e_var (eid 0)))).
-
-Search In _ (_ ++ _).
-Search In _ (_ :: _).
-Print In.
 
 Lemma collect_ctx_expr_refl : forall e C, In C (collect_ctx_expr C e).
 Proof.
