doc/coq/Syntax.v
@@ -21,6 +21,16 @@ Inductive mod_id :=
   | mid (M : nat)
 .
 
+Definition eq_eid id1 id2 :=
+  match id1, id2 with
+  | eid x1, eid x2 => x1 =? x2
+  end.
+
+Definition eq_mid id1 id2 :=
+  match id1, id2 with
+  | mid M1, mid M2 => M1 =? M2
+  end.
+
 Inductive mod_tm :=
   | m_empty
   | m_var (M : mod_id)
@@ -34,9 +44,119 @@ with expr_tm :=
   | e_link (m : mod_tm) (e : expr_tm)
 .
 
+Scheme expr_ind_mut := Induction for expr_tm Sort Prop
+with mod_ind_mut := Induction for mod_tm Sort Prop.
+
 Inductive value : expr_tm -> Prop :=
   | v_fn (x : expr_id) (e : expr_tm) : value (e_lam x e)
 .
 
-Scheme expr_ind_mut := Induction for expr_tm Sort Prop
-with mod_ind_mut := Induction for mod_tm Sort Prop.
+Inductive st_ctx :=
+  | st_c_hole
+  | st_c_lam (x : expr_id) (C : st_ctx)
+  | st_c_lete (x : expr_id) (C : st_ctx)
+  | st_c_letm (M : mod_id) (CM : st_ctx) (C : st_ctx)
+.
+
+Fixpoint st_level (C : st_ctx) : nat :=
+  match C with
+  | st_c_hole => 0
+  | st_c_lam _ C'
+  | st_c_lete _ C' => S (st_level C')
+  | st_c_letm _ _ C' => st_level C'
+  end.
+
+Fixpoint st_ctx_M (C : st_ctx) (M : mod_id) :=
+  match C with
+  | st_c_hole => None
+  | st_c_lam _ C'
+  | st_c_lete _ C' => st_ctx_M C' M
+  | st_c_letm M' CM' C' =>
+    match st_ctx_M C' M with
+    | Some CM => Some CM
+    | None => if eq_mid M M' then Some CM' else None
+    end
+  end.
+
+Fixpoint st_c_plugin (Cout : st_ctx) (Cin : st_ctx) :=
+  match Cout with
+  | st_c_hole => Cin
+  | st_c_lam x C' => st_c_lam x (st_c_plugin C' Cin)
+  | st_c_lete x C' => st_c_lete x (st_c_plugin C' Cin)
+  | st_c_letm M' CM' C' => st_c_letm M' CM' (st_c_plugin C' Cin)
+  end.
+
+Lemma st_c_plugin_assoc : forall C1 C2 C3,
+  st_c_plugin (st_c_plugin C1 C2) C3 =
+  st_c_plugin C1 (st_c_plugin C2 C3). 
+Proof.
+  induction C1; eauto; 
+  intros; simpl; try rewrite IHC1; eauto.
+  rewrite IHC1_2. eauto.
+Qed.
+
+Lemma st_c_plugin_add_level :
+  forall C1 C2, st_level (st_c_plugin C1 C2) = st_level C1 + st_level C2.
+Proof.
+  induction C1; induction C2; intros; simpl; eauto.
+  - assert (RR : st_level (st_c_letm M C2_1 C2_2) = st_level C2_2); eauto.
+    specialize (IHC1 (st_c_letm M C2_1 C2_2)).
+    rewrite IHC1. rewrite RR. eauto.
+  - assert (RR : st_level (st_c_letm M C2_1 C2_2) = st_level C2_2); eauto.
+    specialize (IHC1 (st_c_letm M C2_1 C2_2)).
+    rewrite IHC1. rewrite RR. eauto.
+  - assert (RR : st_level (st_c_letm M0 C2_1 C2_2) = st_level C2_2); eauto.
+    specialize (IHC1_2 (st_c_letm M0 C2_1 C2_2)).
+    rewrite IHC1_2. rewrite RR. eauto.
+Qed.
+
+Notation "Cout '[[|' Cin '|]]'" := (st_c_plugin Cout Cin)
+                              (at level 100, Cin at next level, right associativity).
+
+Notation "'[[||]]'" := (st_c_hole) (at level 100).
+
+(* collect all static contexts reachable from the current configuration *)
+Fixpoint collect_ctx_expr C e :=
+  match e with
+  | e_var x => [C]
+  | e_lam x e' => C :: collect_ctx_expr
+                       (C [[|st_c_lam x ([[||]]) |]]) e'
+  | e_app e1 e2 =>
+    let ctxs1 := collect_ctx_expr C e1 in
+    let ctxs2 := collect_ctx_expr C e2 in
+    ctxs1 ++ ctxs2
+  | e_link m e' =>
+    match collect_ctx_mod C m with
+    | (Some C_m, ctxs_m) => 
+      let ctxs_e := collect_ctx_expr C_m e' in
+      ctxs_m ++ ctxs_e
+    | (None, ctxs_m) => ctxs_m
+    end
+  end
+
+with collect_ctx_mod C m :=
+  match m with
+  | m_empty => (Some C, [C])
+  | m_var M =>
+    match st_ctx_M C M with
+    | Some C_M => (Some C_M, [C ; C_M])
+    | None => (None, [C])
+    end
+  | m_lete x e m' =>
+    let ctxs_e := collect_ctx_expr C e in
+    let (ctx_o, ctxs_m) := collect_ctx_mod 
+                           (C [[| st_c_lete x ([[||]]) |]]) m' in
+    (ctx_o, ctxs_e ++ ctxs_m)
+  | m_letm M m1 m2 =>
+    match collect_ctx_mod C m1 with
+    | (Some C_M, ctxs_m1) => 
+      let (ctx_o, ctxs_m2) := collect_ctx_mod
+                              (C [[| st_c_letm M C_M ([[||]]) |]]) m2 in
+      (ctx_o, ctxs_m1 ++ ctxs_m2)
+    | (None, ctxs_m1) => (None, ctxs_m1)
+    end
+  end.
+
+Compute collect_ctx_expr ([[||]]) (e_app (e_lam (eid 0) (e_var (eid 0)))
+                                  (e_lam (eid 0) (e_var (eid 0)))).
+
